Populating the model definitions

opentheory/examples/memory.ml
@@ -19,7 +19,90 @@ new_type_abbrev("physical_page_address",
 
 new_type_abbrev("physical_address",`:physical_page_address # offset`);;
 
+new_constant ("installed_physical_pages", `:physical_page_address list`);;
+
+let forall_installed_pages_def = new_definition
+  `!p.
+     forall_installed_pages (p : physical_page_address -> bool) =
+     ALL p installed_physical_pages`;;
+
+export_thm forall_installed_pages_def;;
+
+let exists_installed_pages_def = new_definition
+  `!p.
+     exists_installed_pages (p : physical_page_address -> bool) =
+     EX p installed_physical_pages`;;
+
+export_thm exists_installed_pages_def;;
+
+let member_installed_pages_def = new_definition
+  `!ppa.
+     member_installed_pages (ppa : physical_page_address) =
+     MEM ppa installed_physical_pages`;;
+
+export_thm member_installed_pages_def;;
+
+let physical_page_address_lt_def = new_definition
+  `!pdi1 pti1 pdi2 pti2.
+     physical_page_address_lt (pdi1,pti1) (pdi2,pti2) <=>
+     word10_lt pdi1 pdi2 \/ (pdi1 = pdi2 /\ word10_lt pti1 pti2)`;;
+
+export_thm physical_page_address_lt_def;;
+
+let physical_page_address_le_def = new_definition
+  `!vpa1 vpa2.
+     physical_page_address_le vpa1 vpa2 <=>
+     ~physical_page_address_lt vpa2 vpa1`;;
+
+export_thm physical_page_address_le_def;;
+
+let physical_page_address_inc_raw_def = new_definition
+  `!pdi pti.
+     physical_page_address_inc (pdi,pti) =
+     if pti = num_to_word10 1023 then
+       (word10_add pdi (num_to_word10 1), num_to_word10 0)
+     else
+       (pdi, word10_add pti (num_to_word10 1))`;;
+
+let physical_page_address_inc_def = prove
+  (`!pdi pti.
+      (word10_lt pti (num_to_word10 1023) ==>
+       physical_page_address_inc (pdi,pti) =
+       (pdi, word10_add pti (num_to_word10 1))) /\
+      (word10_lt pdi (num_to_word10 1023) ==>
+       physical_page_address_inc (pdi, num_to_word10 1023) =
+       (word10_add pdi (num_to_word10 1), num_to_word10 0))`,
+   REWRITE_TAC [physical_page_address_inc_raw_def] THEN
+   REPEAT GEN_TAC THEN
+   bool_cases_tac `pti = num_to_word10 1023` THENL
+   [ASM_REWRITE_TAC [word10_lt_refl];
+    ASM_REWRITE_TAC []]);;
+
+export_thm physical_page_address_inc_def;;
+
+let physical_page_address_add_def = new_recursive_definition num_RECURSION
+  `(!ppa. physical_page_address_add ppa 0 = ppa) /\
+   (!ppa n.
+      physical_page_address_add ppa (SUC n) =
+      physical_page_address_add (physical_page_address_inc ppa) n)`;;
+
+export_thm physical_page_address_add_def;;
+
+(* Page contents *)
+
 new_type_abbrev("page_data",`:offset -> byte`);;
+
+let zero_page_data_def = new_definition
+  `!off. zero_page_data (off : offset) = num_to_byte 0`;;
+
+export_thm zero_page_data_def;;
+
+let update_page_data_def = new_definition
+  `!off v f off'.
+      update_page_data (off : offset) (v : byte) (f : page_data) off' =
+      if off = off' then v else f off'`;;
+
+export_thm update_page_data_def;;
 
 (* Page directories *)
 
@@ -45,12 +128,90 @@ new_type_abbrev("page_table_index",`:superpage_offset`);;  (*** JEH ***)
 new_type_abbrev("table_page_data",
                 `:page_table_index -> physical_page_address option`);;
 
-(* Virtual pages *)
+(* Virtual addresses *)
 
 new_type_abbrev("virtual_page_address",
                 `:page_directory_index # page_table_index`);;
 
 new_type_abbrev("virtual_address",`:virtual_page_address # offset`);;
+
+let virtual_page_address_lt_def = new_definition
+  `!pdi1 pti1 pdi2 pti2.
+     virtual_page_address_lt (pdi1,pti1) (pdi2,pti2) <=>
+     word10_lt pdi1 pdi2 \/ (pdi1 = pdi2 /\ word10_lt pti1 pti2)`;;
+
+export_thm virtual_page_address_lt_def;;
+
+let virtual_page_address_le_def = new_definition
+  `!vpa1 vpa2.
+     virtual_page_address_le vpa1 vpa2 <=>
+     ~virtual_page_address_lt vpa2 vpa1`;;
+
+export_thm virtual_page_address_le_def;;
+
+let virtual_page_address_inc_raw_def = new_definition
+  `!pdi pti.
+     virtual_page_address_inc (pdi,pti) =
+     if pti = num_to_word10 1023 then
+       (word10_add pdi (num_to_word10 1), num_to_word10 0)
+     else
+       (pdi, word10_add pti (num_to_word10 1))`;;
+
+let virtual_page_address_inc_def = prove
+  (`!pdi pti.
+      (word10_lt pti (num_to_word10 1023) ==>
+       virtual_page_address_inc (pdi,pti) =
+       (pdi, word10_add pti (num_to_word10 1))) /\
+      (word10_lt pdi (num_to_word10 1023) ==>
+       virtual_page_address_inc (pdi, num_to_word10 1023) =
+       (word10_add pdi (num_to_word10 1), num_to_word10 0))`,
+   REWRITE_TAC [virtual_page_address_inc_raw_def] THEN
+   REPEAT GEN_TAC THEN
+   bool_cases_tac `pti = num_to_word10 1023` THENL
+   [ASM_REWRITE_TAC [word10_lt_refl];
+    ASM_REWRITE_TAC []]);;
+
+export_thm virtual_page_address_inc_def;;
+
+let virtual_page_address_add_def = new_recursive_definition num_RECURSION
+  `(!ppa. virtual_page_address_add ppa 0 = ppa) /\
+   (!ppa n.
+      virtual_page_address_add ppa (SUC n) =
+      virtual_page_address_add (virtual_page_address_inc ppa) n)`;;
+
+export_thm virtual_page_address_add_def;;
+
+let user_kernel_boundary_def = new_definition
+  `user_kernel_boundary = (num_to_word10 768, num_to_word10 0)`;;
+
+export_thm user_kernel_boundary_def;;
+
+let is_user_page_address_def = new_definition
+  `!vpa.
+     is_user_page_address vpa =
+     virtual_page_address_lt vpa user_kernel_boundary`;;
+
+export_thm is_user_page_address_def;;
+
+let is_kernel_page_address_def = new_definition
+  `!vpa.
+     is_kernel_page_address vpa <=> ~is_user_page_address vpa`;;
+
+export_thm is_kernel_page_address_def;;
+
+let is_user_address_def = new_definition
+  `!vpa off.
+     is_user_address ((vpa,off) : virtual_address) =
+     is_user_page_address vpa`;;
+
+export_thm is_user_address_def;;
+
+let is_kernel_address_def = new_definition
+  `!vpa off.
+     is_kernel_address ((vpa,off) : virtual_address) =
+     is_kernel_page_address vpa`;;
+
+export_thm is_kernel_address_def;;
 
 (* Page types *)
 
@@ -63,6 +224,30 @@ let page_induct,page_recursion = define_type
 
 export_thm page_induct;;
 export_thm page_recursion;;
+
+let is_normal_def = new_recursive_definition page_recursion
+  `(!pd. is_normal (Environment pd) = F) /\
+   (!pd. is_normal (Normal pd) = T) /\
+   (!pd. is_normal (PageDirectory pd) = F) /\
+   (!pd. is_normal (PageTable pd) = F)`;;
+
+export_thm is_normal_def;;
+
+let is_page_directory_def = new_recursive_definition page_recursion
+  `(!pd. is_page_directory (Environment pd) = F) /\
+   (!pd. is_page_directory (Normal pd) = F) /\
+   (!pd. is_page_directory (PageDirectory pd) = T) /\
+   (!pd. is_page_directory (PageTable pd) = F)`;;
+
+export_thm is_page_directory_def;;
+
+let is_page_table_def = new_recursive_definition page_recursion
+  `(!pd. is_page_table (Environment pd) = F) /\
+   (!pd. is_page_table (Normal pd) = F) /\
+   (!pd. is_page_table (PageDirectory pd) = F) /\
+   (!pd. is_page_table (PageTable pd) = T)`;;
+
+export_thm is_page_table_def;;
 
 (* Regions of physical memory *)
 
@@ -87,6 +272,42 @@ let physical_region_length_def =
 
 export_thm physical_region_length_def;;
 
+let physical_region_to_list_def =
+  new_recursive_definition physical_region_recursion
+  `!s l.
+     physical_region_to_list (PhysicalRegion s l) =
+     MAP (physical_page_address_add s) (interval 0 l)`;;
+
+export_thm physical_region_to_list_def;;
+
+let forall_physical_region_def = new_definition
+  `!p pr.
+     forall_physical_region p pr <=>
+     ALL p (physical_region_to_list pr)`;;
+
+export_thm forall_physical_region_def;;
+
+let exists_physical_region_def = new_definition
+  `!p pr.
+     exists_physical_region p pr <=>
+     EX p (physical_region_to_list pr)`;;
+
+export_thm exists_physical_region_def;;
+
+let member_physical_region_def = new_definition
+  `!ppa pr.
+     member_physical_region ppa pr <=>
+     MEM ppa (physical_region_to_list pr)`;;
+
+export_thm member_physical_region_def;;
+
+let is_physical_subregion_def = new_definition
+  `!pr1 pr2.
+     is_physical_subregion pr1 pr2 <=>
+     forall_physical_region (\ppa. member_physical_region ppa pr2) pr1`;;
+
+export_thm is_physical_subregion_def;;
+
 (* Regions of virtual memory *)
 
 let virtual_region_induct,virtual_region_recursion = define_type
@@ -109,6 +330,56 @@ let virtual_region_length_def =
   `!s l. virtual_region_length (VirtualRegion s l) = l`;;
 
 export_thm virtual_region_length_def;;
+
+let virtual_region_to_list_def =
+  new_recursive_definition virtual_region_recursion
+  `!s l.
+     virtual_region_to_list (VirtualRegion s l) =
+     MAP (virtual_page_address_add s) (interval 0 l)`;;
+
+export_thm virtual_region_to_list_def;;
+
+let forall_virtual_region_def = new_definition
+  `!p vr.
+     forall_virtual_region p vr <=>
+     ALL p (virtual_region_to_list vr)`;;
+
+export_thm forall_virtual_region_def;;
+
+let exists_virtual_region_def = new_definition
+  `!p vr.
+     exists_virtual_region p vr <=>
+     EX p (virtual_region_to_list vr)`;;
+
+export_thm exists_virtual_region_def;;
+
+let member_virtual_region_def = new_definition
+  `!ppa vr.
+     member_virtual_region ppa vr <=>
+     MEM ppa (virtual_region_to_list vr)`;;
+
+export_thm member_virtual_region_def;;
+
+let is_virtual_subregion_def = new_definition
+  `!vr1 vr2.
+     is_virtual_subregion vr1 vr2 <=>
+     forall_virtual_region (\ppa. member_virtual_region ppa vr2) vr1`;;
+
+export_thm is_virtual_subregion_def;;
+
+let is_user_region_def = new_definition
+  `!vr.
+     is_user_region vr <=>
+     forall_virtual_region is_user_page_address vr`;;
+
+export_thm is_user_region_def;;
+
+let is_kernel_region_def = new_definition
+  `!vr.
+     is_kernel_region vr <=>
+     forall_virtual_region is_kernel_page_address vr`;;
+
+export_thm is_kernel_region_def;;
 
 (* The state of the machine *)
 
@@ -281,6 +552,8 @@ new_type_abbrev("output",`:view`);;
 logfile "memory-thm";;
 
 (* Physical pages *)
+
+(* Page contents *)
 
 (* Page directories *)
 
